HelloTypeSystem/Meta/TypingML2.lean
@@ -1,0 +1,73 @@
+import HelloTypeSystem.Meta.EvalML2
+
+namespace HelloTypeSystem.ML2
+open ML2
+
+notation Γ " ⊢ " e " : " τ => Typed Γ e τ
+notation "⊨ " E " : " Γ => Env.compat E Γ
+
+/-!
+# ML2に対する型付け
+-/
+
+/-
+## 型付けの例
+-/
+
+example : [("y", .Int), ⟨"x", .Bool⟩] ⊢ .If "x" ("y" + 1) ("y" - 1) : .Int :=
+  .If
+    (.VarIr .Var)
+    (.Add .Var .Int)
+    (.Sub .Var .Int)
+
+example : [] ⊢ .Let "x" (.LT 3 2) (.Let "y" 5 (.If "x" "y" 2)) : .Int :=
+  .Let
+    (.LT .Int .Int)
+    (.Let
+      (.Int)
+      (.If
+        (.VarIr .Var)
+        (.Var)
+        (.Int)
+      )
+    )
+
+/-!
+## 型安全性
+-/
+
+/--
+TypingML2による型安全性
+-/
+theorem type_safety (compat : (⊨ E : Γ)) : (Γ ⊢ e : τ) → (E ⊢ e ⇓ r) → ∃ v : ML1.Value, r = .inr v ∧ (τ = .Int → ∃ i : Int, v = i) ∧ (τ = .Bool → ∃ b : Bool, v = b)
+  | .Int,          .Int  (i := i) => ⟨i, rfl, fun _ => ⟨i, rfl⟩, Types.noConfusion⟩
+  | .Bool,         .Bool (b := b) => ⟨b, rfl, Types.noConfusion, fun _ => ⟨b, rfl⟩⟩
+  | .Var,          .Var  (v := v) => sorry
+      -- have := if_pos (t := True) (e := False) rfl
+      -- have := compat
+      -- have := if_pos rfl compat
+      -- sorry
+      -- ⟨v, rfl, compat.left rfl⟩
+  -- | .VarIr dt hne, .Var           => sorry -- type_safety (compat.right hne.symm) dt .Var
+  -- | .VarIr (y := y) dt hne, .VarIr (y := y') (v := .Z i) dv hne2 =>
+  --     sorry
+  -- | .VarIr (y := y) dt hne, .VarIr (y := y') (v := v) dv hne2 =>
+  --     compat.elim fun h1 _ =>
+  --       Or.elim (Decidable.em (y' = y))
+  --         (fun heq =>
+  --           have := h1 heq
+  --           sorry)
+  --         (fun _ => sorry)
+        -- ⟨v, rfl, sorry⟩
+      -- have := compat.right sorry
+      -- Or.elim (Decidable.em (y' = y))
+      --   (fun heq =>
+      --     have := compat.right sorry
+      --     have compat' := heq ▸ compat
+      --     have := compat'.left rfl
+      --     have := type_safety sorry dt dv
+      --     sorry)
+      --   (sorry)
+      -- have := compat.right hne
+      -- sorry
+  | _, _ => sorry
